

## Problem 1

Verify that the following construction is a contravariant functor  $F$  from the category of sets to itself: for a set  $A$ ,  $F(A)$  is the power set of  $A$  (that is, the set of all the subsets of  $A$ ), while for a map  $f : A \rightarrow B$ , the induced map  $F(f) : F(B) \rightarrow F(A)$  sends  $X \subset B$  to  $f^{-1}(X) \subset A$ .

*Proof.* Let  $X \subset C$ . Then

$$F(g \circ f)(X) = (g \circ f)^{-1}(X) = f^{-1}(g^{-1}(X)) = F(f)(F(g)(X)).$$

Thus,  $F(g \circ f) = F(f) \circ F(g)$ .

Finally, we check the identity property. Let  $X \subset A$ . Then

$$F(\text{id}_A)(X) = (\text{id}_A)^{-1}(X) = X.$$

Thus,  $F(\text{id}_A) = \text{id}_{F(A)}$ .

Since both properties of **Definition X.1.2** are satisfied,  $F$  is indeed a contravariant functor from the category of sets to itself.  $\square$

## Problem 2

Let  $\mathcal{C}$  be any category. Fix an object  $a \in \mathcal{C}$  and suppose that for any object  $x \in \mathcal{C}$ , the product  $a \times x$  exists. Show that the correspondence

$$x \mapsto a \times x$$

is a functor. (Technically, there is a subtlety here: we know that if a product exists, it is unique up to isomorphism, however, in order to construct a functor, we need to make a specific choice of  $a \times x$  for all  $x$ . It would be better to say that the functor is defined up to a cononical isomorphism, but this detail is usually ignored.)

*Proof.* We need to verify two properties of a functor:

1. For any objects  $x, y, z \in \mathcal{C}$  and any morphisms  $f : x \rightarrow y$  and  $g : y \rightarrow z$ , we have

$$F(g \circ f) = F(g) \circ F(f).$$

2. For any object  $x \in \mathcal{C}$ , we have

$$F(\text{id}_x) = \text{id}_{F(x)}.$$

Let  $f : x \rightarrow y$  and  $g : y \rightarrow z$  be morphisms in  $\mathcal{C}$ . By the universal property of products, there exist unique morphisms  $F(f) : a \times x \rightarrow a \times y$  and  $F(g) : a \times y \rightarrow a \times z$  such that the following diagrams commute:

$$\begin{array}{ccccc} a \times x & \xrightarrow{F(f)} & a \times y & & a \times y & \xrightarrow{F(g)} & a \times z \\ \downarrow \pi_a & & \downarrow \pi_a & & \downarrow \pi_a & & \downarrow \pi_a \\ a & = & a & & a & = & a \end{array}$$

Now, consider the composition  $g \circ f : x \rightarrow z$ . By the universal property of products again, there exists a unique morphism  $F(g \circ f) : a \times x \rightarrow a \times z$  such that the following diagram commutes:

$$\begin{array}{ccc} a \times x & \xrightarrow{F(g \circ f)} & a \times z \\ \downarrow \pi_a & & \downarrow \pi_a \\ a & = & a \end{array}$$

Since both  $F(g) \circ F(f)$  and  $F(g \circ f)$  satisfy the same universal property, by the uniqueness part of the universal property of products, we have

$$F(g \circ f) = F(g) \circ F(f).$$

Finally, we check the identity property. For any object  $x \in \mathcal{C}$ , by the universal property of products, there exists a unique morphism  $F(\text{id}_x) : a \times x \rightarrow a \times x$  such that the following diagram commutes:

$$\begin{array}{ccc} a \times x & \xrightarrow{F(\text{id}_x)} & a \times x \\ \downarrow \pi_a & & \downarrow \pi_a \\ a & = & a \end{array}$$

Since both  $\text{id}_{a \times x}$  and  $F(\text{id}_x)$  satisfy the same universal property, by the uniqueness part of the universal property of products, we have

$$F(\text{id}_x) = \text{id}_{a \times x}.$$

Therefore we have that  $x \mapsto a \times x$  is indeed a functor. □

### Problem 3

Let  $V$  be a linear space and  $P : V \rightarrow V$  be a linear operator such that  $P^2 = P$ . (Operators having this property are called *projectors*.) Show that  $V$  is the internal direct sum of subspaces  $\text{Im}(P)$  and  $\text{Ker}(P)$ .

*Proof.* Notice that for any  $x \in V$  we have that  $x = x - P(x) + P(x)$ . Then  $P(x - P(x)) = P(x) - P^2(x) = 0$ . So we have that  $x - P(x) \in \text{ker}(P)$  and clearly  $P(x) \in \text{im}(P)$ . Now suppose  $x \in \text{ker}(P) \cap \text{im}(P)$ . Fix  $y$  with  $P(x) = y$  then we have that  $0 = P(x) = P^2(x) = P(y)$ . So  $0 = P(x) = P(y) \iff x = y = 0$ . Therefore we have that  $V = \text{ker}(P) \oplus \text{im}(P)$ . □

### Problem 4

Continuing with the previous problem, suppose that  $\dim(V) = n$ . Prove that there exists a basis of  $V$  such that the matrix of  $P$  is of the form  $\text{diag}(1, 1, \dots, 1, 0, 0, \dots, 0)$ . (diag denotes the diagonal matrix with given entries.)

*Proof.* If we fix bases  $\mathcal{B}$  and  $\mathcal{C}$  for  $\text{im}(P)$  and  $\text{ker}(P)$  respectively, then from question 3 we have that  $\mathcal{B} \cup \mathcal{C}$  is a basis for  $V$ . Then for any  $x \in \mathcal{B}$ , fix  $y_x \in V$  such that  $x = P(y_x)$  so we have  $P(x) = P^2(y_x) = P(y_x) = x$ . Then for any  $y \in \mathcal{C}$ , we have  $P(y) = 0$  by definition. Therefore the matrix representation of  $P$  with respect to the basis  $\mathcal{B} \cup \mathcal{C}$  is of the form  $\text{diag}(1, 1, \dots, 1, 0, 0, \dots, 0)$ . □

### Problem 5

Fix  $n$ , and consider the vector space:

$$V = \{p(t) \in \mathbb{R}[t] : \deg(p) \leq n\}$$

over  $\mathbb{R}$ . Fix  $n + 1$  numbers  $a_0, \dots, a_n \in \mathbb{R}$  and consider the map

$$\phi : V \rightarrow \mathbb{R}^{n+1}; \quad \phi(p) = (p(a_0), \dots, p(a_n)).$$

Show that  $\phi$  is invertible (and therefore an isomorphism of vector spaces) if and only if  $a_i$ 's are all distinct.

*Proof.* ( $\Leftarrow$ ) Suppose the  $a_i$ 's are all distinct. We first show that  $\phi$  is injective. Suppose  $\phi(p) = \phi(q)$  for some  $p, q \in V$ . Then we have that  $p(a_i) = q(a_i)$  for all  $0 \leq i \leq n$ . Thus, the polynomial  $r(t) = p(t) - q(t)$  has  $n + 1$  distinct roots  $a_0, a_1, \dots, a_n$ . Since  $\deg(r) \leq n$ , we must have  $r(t) \equiv 0$ , which implies that  $p(t) = q(t)$ . Therefore,  $\phi$  is injective.

To show that  $\phi$  is surjective, let  $(b_0, b_1, \dots, b_n) \in \mathbb{R}^{n+1}$  be any vector. We need to find a polynomial  $p(t) \in V$  such that  $\phi(p) = (b_0, b_1, \dots, b_n)$ . This is equivalent to solving the system of equations:

$$p(a_i) = b_i \quad \text{for } i = 0, 1, \dots, n.$$

Since the  $a_i$ 's are distinct, we have:

$$p(t) = \sum_{i=0}^n b_i \prod_{\substack{0 \leq j \leq n \\ j \neq i}} \frac{t - a_j}{a_i - a_j}$$

is a polynomial of degree at most  $n$  that satisfies the above equations. Thus,  $\phi$  is surjective. Since  $\phi$  is both injective and surjective, it is invertible.

( $\Rightarrow$ ) Now suppose that the  $a_i$ 's are not all distinct. Without loss of generality, assume that  $a_0 = a_1$ . We will show that  $\phi$  is not injective. Consider the polynomial  $p(t) = t - a_0$ . Then we have:

$$\phi(p) = (p(a_0), p(a_1), \dots, p(a_n)) = (0, 0, p(a_2), \dots, p(a_n)).$$

Now consider the zero polynomial  $q(t) = 0$ . We have:

$$\phi(q) = (q(a_0), q(a_1), \dots, q(a_n)) = (0, 0, 0, \dots, 0).$$

Since  $\phi(p) \neq \phi(q)$ , we have found two distinct polynomials  $p$  and  $q$  such that  $\phi(p) = \phi(q)$ . Therefore,  $\phi$  is not injective, and hence not invertible. □

### Problem 6

Let  $V$  be a vector space over a field  $K$ . A (linear) functional on  $V$  is a linear operator  $\phi : V \rightarrow K$ . Show that if two functionals  $\phi, \psi : V \rightarrow K$  satisfy  $\ker(\phi) \subset \ker(\psi)$ , then there exists  $a \in K$  such that  $\psi = a\phi$ . (If you need to, you can assume that  $V$  is finite-dimensional, but it should not be necessary.)

*Proof.* If  $\phi = 0$  then  $\ker \phi = V$ , so  $\ker \psi = V$  and hence  $\psi = 0$ ; take  $a = 0$ . Otherwise pick  $v_0 \in V$  with  $\phi(v_0) = 1$  and set  $a = \psi(v_0)$ . For any  $v \in V$  put

$$u := v - \phi(v)v_0.$$

Then  $\phi(u) = \phi(v) - \phi(v)\phi(v_0) = 0$ , so  $u \in \ker \phi \subset \ker \psi$ , hence  $\psi(u) = 0$ . Therefore

$$0 = \psi(u) = \psi(v) - \phi(v)\psi(v_0) = \psi(v) - a\phi(v),$$

so  $\psi(v) = a\phi(v)$  for all  $v \in V$ . Uniqueness of  $a$  follows since  $a = \psi(v_0)$ . □

### Problem 7

Let  $K$  be a field and  $L \subset K$  be a smaller field (e.g.,  $L = \mathbb{R}$  and  $K = \mathbb{C}$ ). Given a  $K$ -vector space  $V$ , we can also consider it as a  $L$ -vector space, so we get two notions of dimension: as a vector space over  $K$  and as a vector space over  $L$ . Denote them by  $\dim_K V$  and  $\dim_L V$ , respectively. Show that

$$\dim_L V = (\dim_K V) \cdot (\dim_L K).$$

*Proof.* Let  $\{v_1, v_2, \dots, v_n\}$  be a basis for  $V$  over  $K$  and let  $\{k_1, k_2, \dots, k_m\}$  be a basis for  $K$  over  $L$ . We claim that the set

$$\{k_i v_j : 1 \leq i \leq m, 1 \leq j \leq n\}$$

is a basis for  $V$  over  $L$ .

First we show that this set spans  $V$  over  $L$ . Take any  $v \in V$ . Since  $\{v_1, v_2, \dots, v_n\}$  is a basis for  $V$  over  $K$ , we can write

$$v = a_1 v_1 + a_2 v_2 + \dots + a_n v_n$$

for some  $a_i \in K$ . Each  $a_i$  can be expressed as a linear combination of the basis elements of  $K$  over  $L$ , i.e.,

$$a_i = b_{i1} k_1 + b_{i2} k_2 + \dots + b_{im} k_m$$

for some  $b_{ij} \in L$ . Substituting this back into the expression for  $v$ , we get

$$v = \sum_{j=1}^n \left( \sum_{i=1}^m b_{ij} k_i \right) v_j = \sum_{i=1}^m \sum_{j=1}^n b_{ij} (k_i v_j),$$

which shows that  $v$  can be expressed as an  $L$ -linear combination of the elements in our set.

Next, we show that the set is linearly independent over  $L$ . Suppose we have

$$\sum_{i=1}^m \sum_{j=1}^n c_{ij} (k_i v_j) = 0$$

for some  $c_{ij} \in L$ . Rearranging gives

$$\sum_{j=1}^n \left( \sum_{i=1}^m c_{ij} k_i \right) v_j = 0.$$

Since  $\{v_1, v_2, \dots, v_n\}$  is a basis for  $V$  over  $K$ , the coefficients must all be zero, i.e.,

$$\sum_{i=1}^m c_{ij} k_i = 0 \quad \forall j.$$

But since  $\{k_1, k_2, \dots, k_m\}$  is a basis for  $K$  over  $L$ , we have that  $c_{ij} = 0$  for all  $i, j$ . This shows that our set is linearly independent over  $L$ .

Since we have shown that the set spans  $V$  over  $L$  and is linearly independent over  $L$ , we conclude that it is a basis for  $V$  over  $L$ . Therefore we have

$$\dim_L V = m \cdot n = (\dim_K V) \cdot (\dim_L K).$$

□